src/MetaTheory.v
@@ -1,0 +1,336 @@
+(* Celsius project *)
+(* Clément Blaudeau - LAMP@EPFL 2021 *)
+(** Store typing *)
+
+From Celsius Require Export Typing LibTactics Tactics Reachability.
+Require Import Coq.ssr.ssreflect Coq.ssr.ssrbool Coq.Lists.List Coq.micromega.Psatz Ensembles Coq.Program.Tactics.
+(* Import ListNotations. *)
+(* Open Scope nat_scope. *)
+
+
+(** * Main definitions *)
+
+(** ** Monotonicity *)
+Definition monotonicity Σ1 Σ2 :=
+  forall l, l < dom Σ1 -> (exists T1 T2, getType Σ1 l = Some T1 /\ getType Σ2 l = Some T2 /\ T2 <: T1).
+Notation "Σ1 ≼ Σ2" := (monotonicity Σ1 Σ2) (at level 60).
+
+(** ** Authority *)
+Definition authority Σ1 Σ2 :=
+  forall l, l < dom Σ1 -> (exists T, getType Σ1 l = Some T /\ getType Σ2 l = Some T).
+Notation "Σ1 ▷ Σ2" := (authority Σ1 Σ2) (at level 60).
+
+(** ** Value typing (with variants) *)
+
+Inductive value_typing : StoreTyping -> Loc -> Tpe -> Prop :=
+| vt_sub : forall Σ l (T1 T2: Tpe),
+    getType Σ l = Some T1 ->
+    (T1 <: T2) -> value_typing Σ l T2.
+Global Instance notation_value_typing_Tpe : notation_dash_colon StoreTyping Loc Tpe :=
+  { dash_colon_ := value_typing }.
+Global Hint Unfold notation_value_typing_Tpe: notations.
+
+Definition value_typing_mode Σ l μ :=
+  exists C, Σ ⊨ l : (C, μ).
+Global Instance notation_value_typing_Mode : notation_dash_colon StoreTyping Loc Mode :=
+  { dash_colon_ := value_typing_mode }.
+Global Hint Unfold notation_value_typing_Mode: notations.
+
+Definition value_typing_cln Σ l C :=
+  exists μ, Σ ⊨ l : (C, μ).
+Global Instance notation_value_typing_ClN : notation_dash_colon StoreTyping Loc ClN :=
+  { dash_colon_ := value_typing_cln }.
+Global Hint Unfold notation_value_typing_ClN: notations.
+
+Definition value_typing_locset Σ L (μ:Mode) :=
+  forall (l: Loc), (In Loc L l) -> Σ ⊨ l : μ.
+Global Instance notation_value_typing_LocSet : notation_dash_colon StoreTyping LocSet Mode :=
+  { dash_colon_ := value_typing_locset }.
+Global Hint Unfold notation_value_typing_LocSet: notations.
+
+(** ** Stackability *)
+Definition stackability_st (Σ1 Σ2: StoreTyping) :=
+  forall l, l < dom Σ2 -> (Σ2 ⊨ l : warm) \/ (l < dom Σ1).
+Global Instance notation_stackability_StoreTyping : notation_stackability StoreTyping :=
+  { stackability_ := stackability_st }.
+Global Hint Unfold notation_stackability_StoreTyping : notations.
+
+(** ** Object typing **)
+Inductive object_typing : StoreTyping -> Obj -> Tpe -> Prop :=
+| ot_hot : forall Σ C ω,
+  (exists args flds mtds,
+    (ct C = Some (class args flds mtds)) /\
+      (forall f, f < length ω ->
+            exists v D μ,
+              getVal ω f = Some v /\
+              fieldType C f = Some (D, μ) /\
+              Σ ⊨ v : (D, hot))) ->
+    object_typing Σ (C,ω) (C, hot)
+| ot_warm : forall Σ C ω,
+    (exists args flds mtds,
+        (ct C = Some (class args flds mtds)) /\
+          (forall f, f < length flds ->
+                exists v D μ,
+                  getVal ω f = Some v ->
+                  fieldType C f = Some (D, μ) ->
+                  Σ ⊨ v : (D, μ))) ->
+    object_typing Σ (C,ω) (C, warm)
+| ot_cool : forall Σ C ω,
+    (forall f v T μ,
+        getVal ω f = Some v ->
+        fieldType C f = Some (T, μ) ->
+        Σ ⊨ v : (T, μ)) ->
+    object_typing Σ (C,ω) (C, cool (dom ω))
+| ot_cold : forall Σ C ω,
+    (forall f v T μ,
+        getVal ω f = Some v ->
+        fieldType C f = Some (T, μ) ->
+        Σ ⊨ v : (T, μ)) ->
+    object_typing Σ (C,ω) (C, cold).
+
+Global Instance notation_object_typing : notation_dash_colon StoreTyping Obj Tpe :=
+  { dash_colon_ := object_typing }.
+Global Hint Unfold notation_object_typing: notations.
+
+(** ** Store_typing *)
+(** Here is the link between the abstract environment of types and the store used in execution *)
+Definition store_typing (Σ: StoreTyping) (σ: Store) :=
+  forall l, l < dom Σ ->
+       exists C ω μ, getObj σ l = Some (C,ω) /\
+                  getType Σ l = Some (C, μ) /\
+                  Σ ⊨ (C, ω) : (C, μ).
+Global Instance notation_store_typing: notation_dash StoreTyping Store :=
+  { dash_ := store_typing }.
+Global Hint Unfold notation_store_typing: notations.
+
+(** ** Environment typing *)
+Inductive env_typing : EnvTyping -> StoreTyping -> Env -> Prop :=
+| et_nil : forall Σ, env_typing nil Σ nil
+| et_cons : forall Γ Σ ρ l T,
+    env_typing Γ Σ ρ ->
+    Σ ⊨ l : T ->
+    env_typing (T :: Γ) Σ (l :: ρ).
+Global Instance notation_env_typing: notation_dash (EnvTyping * StoreTyping) Env :=
+  { dash_ := fun a b => env_typing (fst a) (snd a) b }.
+Global Hint Unfold notation_env_typing: notations.
+
+Implicit Type l : Loc.
+Implicit Type T : Tpe.
+Implicit Type Σ : StoreTyping.
+
+(** * Tactics *)
+Ltac meta :=
+  repeat
+    match goal with
+    | H: getObj ?σ ?l = Some ?O,
+        H': getObj ?σ ?l = Some ?O' |- _ => rewrite H' in H; inverts H
+    | H: getType ?Σ ?l = Some ?T,
+        H': getType ?Σ ?l = Some ?T' |- _ => rewrite H' in H; inverts H
+    | H: getVal ?ρ ?f = Some ?l,
+        H': getVal ?ρ ?f = Some ?l' |- _ => rewrite H' in H; inverts H
+    | H: getType ?Σ ?l = Some ?T |- _ =>
+        let fresh := fresh "H__dom" in
+        add_hypothesis fresh (getType_dom Σ l T H)
+    | H: getVal ?ρ ?f = Some ?l |- _ =>
+        let fresh := fresh "H__dom" in
+        add_hypothesis fresh (getVal_dom ρ f l H)
+    | H: ?Σ ⊨ ?l : ?x |- _ =>
+        match type of l with
+        | Loc => match type of x with
+                | Mode => let C := fresh "C" in destruct H as [C H]
+                | (ClN*Mode)%type =>
+                    inverts H
+                end
+        end
+    | o:Obj |- _ => let C := fresh "C" in
+                  let ω := fresh "ω" in
+                  destruct o as [C ω]
+    | T:Tpe |- _ => let C := fresh "C" in
+                  let μ := fresh "μ" in
+                  destruct T as [C μ]
+    | H: ?μ ⊑ hot |- _ =>
+        let H__eq := fresh "H__eq" in
+        assert (H__eq: μ = hot) by (invert H; steps); subst;
+        clear H
+    | H: (?C, ?μ) <: (?C', ?μ') |- _ => inverts H
+    end ; sort;
+  try lia.
+
+(** * Monotonicity results *)
+
+Lemma monotonicity_dom :
+  forall Σ1 Σ2, Σ1 ≼ Σ2 -> dom Σ1 <= dom Σ2.
+Proof with meta.
+  intros.
+  edestruct PeanoNat.Nat.le_gt_cases; eauto.
+  destruct (dom Σ1) eqn:E; steps; try lia ...
+  specialize (H n) ...
+  destruct H; steps ...
+Qed.
+Global Hint Resolve monotonicity_dom: typ.
+
+Ltac monotonicity_dom :=
+  repeat match goal with
+         | H : ?Σ ≼ ?Σ' |- _ =>
+             let Hf := fresh "H__dom" in
+             add_hypothesis Hf (monotonicity_dom Σ Σ' H)
+         end.
+
+Lemma value_typing_dom : forall Σ l T,
+    Σ ⊨ l : T -> l < dom Σ.
+Proof with meta.
+  intros ...
+Qed.
+Global Hint Resolve value_typing_dom: typ.
+
+Lemma value_typing_monotonicity: forall (Σ1 Σ2: StoreTyping) l T,
+    Σ1 ≼ Σ2 -> Σ1 ⊨ l : T -> Σ2 ⊨ l : T.
+Proof with (meta; eauto with lia typ).
+  intros ...
+  specialize (H l H0) as [T1 [T2 [Hs1 [Hs2 H__sub]]]] ...
+  eapply vt_sub ...
+Qed.
+Global Hint Resolve value_typing_monotonicity: typ.
+
+Lemma env_typing_monotonicity: forall (Σ1 Σ2: StoreTyping) (Γ:EnvTyping) (ρ: Env),
+    Σ1 ≼ Σ2 -> (Γ, Σ1) ⊨ ρ -> (Γ, Σ2) ⊨ ρ.
+Proof.
+  intros.
+  autounfold with notations in H0. simpl in H0.
+  induction H0.
+  - steps.
+  - specialize (IHenv_typing H).
+    apply et_cons; steps; eauto with typ.
+Qed.
+Global Hint Resolve env_typing_monotonicity: typ.
+
+Lemma object_typing_monotonicity: forall (Σ1 Σ2: StoreTyping) (o: Obj) T,
+    Σ1 ≼ Σ2 -> Σ1 ⊨ o : T -> Σ2 ⊨ o : T.
+Proof with (meta; eauto with lia typ).
+  intros ...
+  autounfold with notations in H0.
+  inversion H0; steps.
+  - apply ot_hot.
+    exists args, flds, mtds; split => //.
+    intros.
+    specialize (H3 f H1); steps.
+    exists v, D, μ; steps ...
+  - apply ot_warm.
+    exists args, flds, mtds; split => //.
+    intros.
+    specialize (H3 f H1); steps.
+    exists v, D, μ; steps ...
+  - apply ot_cool.
+    intros.
+    specialize (H3 f v T μ H1 H2); steps ...
+  - apply ot_cold.
+    intros.
+    specialize (H3 f v T μ H1 H2); steps ...
+Qed.
+Global Hint Resolve object_typing_monotonicity: typ.
+
+Lemma mn_refl: forall Σ,
+    Σ ≼ Σ.
+Proof with (meta; eauto with lia typ).
+  intros Σ l; steps ...
+  destruct (getType Σ l) eqn:H__l ...
+  exfalso.
+  apply nth_error_Some in H ...
+Qed.
+Global Hint Resolve mn_refl : typ.
+
+Lemma mn_trans: forall Σ1 Σ2 Σ3,
+    Σ1 ≼ Σ2 -> Σ2 ≼ Σ3 -> Σ1 ≼ Σ3.
+Proof with (meta; eauto with lia typ).
+  intros.
+  intros l; steps.
+  monotonicity_dom.
+  specialize (H l H1); steps.
+  specialize (H0 l) as [ ]; steps; try lia.
+  exists T1 T0; steps ...
+Qed.
+Global Hint Resolve mn_trans: typ.
+
+Lemma env_regularity: forall Γ Σ ρ x U T,
+    (Γ, Σ) ⊨ ρ ->
+    (Γ, U) ⊢ (var x) : T ->
+    exists l, getVal ρ x = Some l /\ Σ ⊨ l : T.
+Proof.
+  intros ...
+  remember (var x) as e.
+  induction H0; try congruence.
+  - specialize (IHT_Expr H Heqe) as [l [H__val Ht]].
+    exists l; steps.
+    inverts Ht.
+    eapply vt_sub; eauto with typ.
+  - steps.
+    gen U x.
+    autounfold with notations in H. simpl in *.
+    induction H; intros; destruct x; steps; eauto.
+Qed.
+
+Lemma hot_transitivity : forall (Σ: StoreTyping) (σ: Store) l l',
+    Σ ⊨ l : hot ->
+    Σ ⊨ σ ->
+    σ ⊨ l ⇝ l' ->
+    Σ ⊨ l' : hot.
+Proof with (meta; eauto with lia typ).
+  intros.
+  gen Σ.
+  induction H1; steps ...
+  specialize (H3 l0) as [ ] ...
+  steps ...
+  inverts H8; steps ...
+  specialize (H9 f) as [ ] ; steps...
+  eexists; steps ...
+Qed.
+
+
+(** ** Authority results *)
+
+Lemma aty_refl: forall Σ, Σ ▷ Σ.
+Proof with (meta; eauto with typ lia).
+  intros Σ l H.
+  destruct (getType Σ l) eqn:E; eauto.
+  exfalso;
+  eapply nth_error_Some; unfold getType in *; eauto.
+Qed.
+
+Lemma aty_trans: forall Σ1 Σ2 Σ3,
+    Σ1 ▷ Σ2 ->
+    dom Σ1 <= dom Σ2 ->
+    Σ2 ▷ Σ3 ->
+    Σ1 ▷ Σ3.
+Proof with steps.
+  intros. intros l ...
+  specialize (H l) ...
+  specialize (H1 l) ...
+  exists T; split ...
+  destruct H1 as [T' [ ]];
+    eauto with lia.
+Qed.
+
+(** ** Stackability results *)
+
+Lemma stk_st_refl: forall Σ, Σ ≪ Σ.
+Proof.
+  intros Σ l H. right => //.
+Qed.
+
+Lemma stk_st_trans: forall Σ1 Σ2 Σ3,
+    Σ1 ≪ Σ2 ->
+    Σ2 ≪ Σ3 ->
+    Σ2 ≼ Σ3 ->
+    Σ1 ≪ Σ3.
+Proof.
+  intros.
+  intros l ?.
+  specialize (H0 l) as [ ]; eauto.
+  specialize (H l H0) as [ ]; eauto.
+  inverts H.
+  inverts H3.
+  left.
+  specialize (H1 l) as [ ]; steps.
+  rewrite H3 in H; steps.
+  exists x, T2; steps; eauto with typ.
+Qed.
